%2multibyte Version: 5.50.0.2960 CodePage: 936
\documentclass{article}%
\usepackage{amsmath}
\usepackage{amsfonts}
\usepackage{amssymb}
\usepackage{graphicx}%
\setcounter{MaxMatrixCols}{30}
%TCIDATA{OutputFilter=latex2.dll}
%TCIDATA{Version=5.50.0.2960}
%TCIDATA{Codepage=936}
%TCIDATA{CSTFile=40 LaTeX article.cst}
%TCIDATA{Created=Sunday, November 08, 2015 20:36:30}
%TCIDATA{LastRevised=Sunday, November 08, 2015 21:27:55}
%TCIDATA{<META NAME="GraphicsSave" CONTENT="32">}
%TCIDATA{<META NAME="SaveForMode" CONTENT="1">}
%TCIDATA{BibliographyScheme=Manual}
%TCIDATA{<META NAME="DocumentShell" CONTENT="Standard LaTeX\Blank - Standard LaTeX Article">}
%BeginMSIPreambleData
\providecommand{\U}[1]{\protect\rule{.1in}{.1in}}
%EndMSIPreambleData
\newtheorem{theorem}{Theorem}
\newtheorem{acknowledgement}[theorem]{Acknowledgement}
\newtheorem{algorithm}[theorem]{Algorithm}
\newtheorem{axiom}[theorem]{Axiom}
\newtheorem{case}[theorem]{Case}
\newtheorem{claim}[theorem]{Claim}
\newtheorem{conclusion}[theorem]{Conclusion}
\newtheorem{condition}[theorem]{Condition}
\newtheorem{conjecture}[theorem]{Conjecture}
\newtheorem{corollary}[theorem]{Corollary}
\newtheorem{criterion}[theorem]{Criterion}
\newtheorem{definition}[theorem]{Definition}
\newtheorem{example}[theorem]{Example}
\newtheorem{exercise}[theorem]{Exercise}
\newtheorem{lemma}[theorem]{Lemma}
\newtheorem{notation}[theorem]{Notation}
\newtheorem{problem}[theorem]{Problem}
\newtheorem{proposition}[theorem]{Proposition}
\newtheorem{remark}[theorem]{Remark}
\newtheorem{solution}[theorem]{Solution}
\newtheorem{summary}[theorem]{Summary}
\newenvironment{proof}[1][Proof]{\noindent\textbf{#1.} }{\ \rule{0.5em}{0.5em}}
\begin{document}
PDE%
\[
\frac{\partial u}{\partial t}+\frac{\partial u}{\partial x}=0
\]


First-order upwind scheme%

\[
\frac{u_{j}^{n+1}-u_{j}^{n}}{\Delta t}=\frac{u_{j}^{n}-u_{j-1}^{n}}{\Delta x}%
\]%
\[
u_{j}^{n+1}=u_{j}^{n}-c\left(  u_{j}^{n}-u_{j-1}^{n}\right)
\]%
\[
c=\frac{\Delta t}{\Delta x}%
\]


Implicit scheme%
\[
\frac{u_{j}^{n+1}-u_{j}^{n}}{\Delta t}=\frac{u_{j+1}^{n+1}-u_{j-1}^{n+1}%
}{2\Delta x}%
\]%
\[
-\frac{c}{2}u_{j-1}^{n+1}+u_{j}^{n+1}+\frac{c}{2}u_{j+1}^{n+1}=u_{j}^{n}%
\]
%

\[
c=\frac{\Delta t}{\Delta x}%
\]


Lax scheme%
\[
\frac{u_{j}^{n+1}-\frac{1}{2}\left(  u_{j+1}^{n}+u_{j-1}^{n}\right)  }{\Delta
t}=\frac{u_{j+1}^{n}-u_{j-1}^{n}}{2\Delta x}%
\]%
\[
u_{j}^{n+1}=\frac{1}{2}\left(  1-c\right)  u_{j+1}^{n}+\frac{1}{2}\left(
1+c\right)  u_{j-1}^{n}%
\]


Lax-wndroff scheme%
\[
\frac{u_{j}^{n+1}-u_{j}^{n}}{\Delta t}+\frac{u_{j+1}^{n}-u_{j-1}^{n}}{2\Delta
x}=\frac{1}{2}\Delta t\frac{u_{j+1}^{n}-2u_{j}^{n}+u_{j-1}^{n}}{\Delta x^{2}}%
\]%
\begin{align*}
u_{j}^{n+1}  & =u_{j}^{n}-\frac{1}{2}c\left(  u_{j+1}^{n}-u_{j-1}^{n}\right)
+\frac{1}{2}c^{2}\left(  u_{j+1}^{n}-2u_{j}^{n}+u_{j-1}^{n}\right)  \\
& =\left(  1-c^{2}\right)  u_{j}^{n}+\frac{1}{2}c^{2}u_{j+1}^{n}-\frac{1}%
{2}cu_{j+1}^{n}+\frac{1}{2}c^{2}u_{j-1}^{n}+\frac{1}{2}cu_{j-1}^{n}\\
& =\left(  1-c^{2}\right)  u_{j}^{n}+\frac{1}{2}c\left(  c-1\right)
u_{j+1}^{n}+\frac{1}{2}c\left(  c+1\right)  u_{j-1}^{n}%
\end{align*}


Leap-frog scheme%
\[
\frac{u_{j}^{n+1}-u_{j}^{n-1}}{2\Delta t}=\frac{u_{j+1}^{n}-u_{j-1}^{n}%
}{2\Delta x}%
\]%
\[
u_{j}^{n+1}=u_{j}^{n-1}-c\left(  u_{j+1}^{n}-u_{j-1}^{n}\right)
\]



\end{document}